common/Memtype.v
@@ -47,42 +47,10 @@ Being empty is represented by the absence of any permission.
 *)
 
 Inductive permission: Type :=
-  | Freeable: permission
-  | Writable: permission
-  | Readable: permission
-  | Nonempty: permission.
-
-(** In the list, each permission implies the other permissions further down the
-    list.  We reflect this fact by the following order over permissions. *)
-
-Inductive perm_order: permission -> permission -> Prop :=
-  | perm_refl:  forall p, perm_order p p
-  | perm_F_any: forall p, perm_order Freeable p
-  | perm_W_R:   perm_order Writable Readable
-  | perm_any_N: forall p, perm_order p Nonempty.
-
-Global Hint Constructors perm_order: mem.
-
-Lemma perm_order_trans:
-  forall p1 p2 p3, perm_order p1 p2 -> perm_order p2 p3 -> perm_order p1 p3.
-Proof.
-  intros. inv H; inv H0; constructor.
-Qed.
-
-(** Each address has not one, but two permissions associated
-  with it.  The first is the current permission.  It governs whether
-  operations (load, store, free, etc) over this address succeed or
-  not.  The other is the maximal permission.  It is always at least as
-  strong as the current permission.  Once a block is allocated, the
-  maximal permission of an address within this block can only
-  decrease, as a result of [free] or [drop_perm] operations, or of
-  external calls.  In contrast, the current permission of an address
-  can be temporarily lowered by an external call, then raised again by
-  another external call. *)
-
-Inductive perm_kind: Type :=
-  | Max: perm_kind
-  | Cur: perm_kind.
+| Live: permission          (* Allocated: reads and writes always succeed *)
+| MostlyDead: permission    (* Not allocated, but not shadowed by compiler data *) 
+| Dead: permission          (* Shadowed by compiler data *)
+.
 
 Module Type MEM.
 
@@ -101,7 +69,7 @@ Parameter empty: mem.
   Returns a pair [(m', b)] of the updated memory state [m'] and
   the identifier [b] of the newly-allocated block.
   Note that [alloc] never fails: we are modeling an infinite memory. *)
-Parameter alloc: forall (m: mem) (lo hi: Z), mem * block.
+Parameter alloc: forall (m: mem) (lo hi: Z), option (mem * Z * Z).
 
 (** [free m b lo hi] frees (deallocates) the range of offsets from [lo]
   included to [hi] excluded in block [b].  Returns the updated memory
@@ -157,104 +125,90 @@ Fixpoint free_list (m: mem) (l: list (block * Z * Z)) {struct l}: option mem :=
       end
   end.
 
-(** [drop_perm m b lo hi p] sets the permissions of the byte range
-    [(b, lo) ... (b, hi - 1)] to [p].  These bytes must have [Freeable] permissions
-    in the initial memory state [m].
-    Returns updated memory state, or [None] if insufficient permissions. *)
-
-Parameter drop_perm: forall (m: mem) (b: block) (lo hi: Z) (p: permission), option mem.
-
 (** * Permissions, block validity, access validity, and bounds *)
 
 (** The next block of a memory state is the block identifier for the
   next allocation.  It increases by one at each allocation.
-  Block identifiers below [nextblock] are said to be valid, meaning
-  that they have been allocated previously.  Block identifiers above
-  [nextblock] are fresh or invalid, i.e. not yet allocated.  Note that
+  Block identifiers below [nextblock] are said to be valid if they are
+  not freed. Block identifiers above [nextblock] are fresh or invalid,
+  i.e. not yet allocated.  Note that
   a block identifier remains valid after a [free] operation over this
   block. *)
 
-Parameter nextblock: mem -> block.
+Parameter nextblock : mem -> block.
 
-Definition valid_block (m: mem) (b: block) := Plt b (nextblock m).
+Parameter valid_block : mem -> block -> Prop.
+
+Parameter in_block : mem -> block -> Z -> Prop.
 
 Axiom valid_not_valid_diff:
   forall m b b', valid_block m b -> ~(valid_block m b') -> b <> b'.
 
 (** [perm m b ofs k p] holds if the address [b, ofs] in memory state [m]
-  has permission [p]: one of freeable, writable, readable, and nonempty.
-  If the address is empty, [perm m b ofs p] is false for all values of [p].
-  [k] is the kind of permission we are interested in: either the current
-  permissions or the maximal permissions. *)
-Parameter perm: forall (m: mem) (b: block) (ofs: Z) (k: perm_kind) (p: permission), Prop.
-
-(** Logical implications between permissions *)
-
-Axiom perm_implies:
-  forall m b ofs k p1 p2, perm m b ofs k p1 -> perm_order p1 p2 -> perm m b ofs k p2.
-
-(** The current permission is always less than or equal to the maximal permission. *)
-
-Axiom perm_cur_max:
-  forall m b ofs p, perm m b ofs Cur p -> perm m b ofs Max p.
-Axiom perm_cur:
-  forall m b ofs k p, perm m b ofs Cur p -> perm m b ofs k p.
-Axiom perm_max:
-  forall m b ofs k p, perm m b ofs k p -> perm m b ofs Max p.
-
-(** Having a (nonempty) permission implies that the block is valid.
-  In other words, invalid blocks, not yet allocated, are all empty. *)
-Axiom perm_valid_block:
-  forall m b ofs k p, perm m b ofs k p -> valid_block m b.
-
-(* Unused?
-(** The [Mem.perm] predicate is decidable. *)
-Axiom perm_dec:
-  forall m b ofs k p, {perm m b ofs k p} + {~ perm m b ofs k p}.
-*)
+  has permission [p]. *)
+Parameter perm: forall (m: mem) (b: block) (ofs: Z) (p: permission), Prop.
 
 (** [range_perm m b lo hi p] holds iff the addresses [b, lo] to [b, hi-1]
-  all have permission [p] of kind [k]. *)
-Definition range_perm (m: mem) (b: block) (lo hi: Z) (k: perm_kind) (p: permission) : Prop :=
-  forall ofs, lo <= ofs < hi -> perm m b ofs k p.
+  all have permission [p]. *)
+Definition range_perm (m: mem) (b: block) (lo hi: Z) (p: permission) : Prop :=
+  forall ofs, lo <= ofs < hi -> perm m b ofs p.
 
-Axiom range_perm_implies:
-  forall m b lo hi k p1 p2,
-  range_perm m b lo hi k p1 -> perm_order p1 p2 -> range_perm m b lo hi k p2.
+Definition range_perm_neg (m: mem) (b: block) (lo hi: Z) (p: permission) : Prop :=
+  forall ofs, lo <= ofs < hi -> ~ perm m b ofs p.
 
-(** An access to a memory quantity [chunk] at address [b, ofs] with
-  permission [p] is valid in [m] if the accessed addresses all have
-  current permission [p] and moreover the offset is properly aligned. *)
-Definition valid_access (m: mem) (chunk: memory_chunk) (b: block) (ofs: Z) (p: permission): Prop :=
-  range_perm m b ofs (ofs + size_chunk chunk) Cur p
+(** An access to a memory quantity [chunk] at address [b, ofs]
+  is valid in [m] if the accessed addresses all have
+  permission [Live] and moreover the offset is properly aligned. *)
+Definition valid_access (m: mem) (chunk: memory_chunk) (b: block) (ofs: Z) : Prop :=
+  range_perm m b ofs (ofs + size_chunk chunk) Live
   /\ (align_chunk chunk | ofs).
-
-Axiom valid_access_implies:
-  forall m chunk b ofs p1 p2,
-  valid_access m chunk b ofs p1 -> perm_order p1 p2 ->
-  valid_access m chunk b ofs p2.
 
 Axiom valid_access_valid_block:
   forall m chunk b ofs,
-  valid_access m chunk b ofs Nonempty ->
-  valid_block m b.
+    valid_access m chunk b ofs ->
+    exists b',
+      valid_block m b' /\ in_block m b' ofs.
+
+Axiom valid_block_valid_access:
+  forall m chunk b b' ofs,
+    valid_block m b' ->
+    in_block m b' ofs ->
+    valid_access m chunk b ofs.
 
 Axiom valid_access_perm:
-  forall m chunk b ofs k p,
-  valid_access m chunk b ofs p ->
-  perm m b ofs k p.
+  forall m chunk b ofs,
+  valid_access m chunk b ofs ->
+  perm m b ofs Live.
+
+(** An access to a memory quantity [chunk] at address [b, ofs] with
+  permission [p] is allowed in [m] if none of the accessed addresses have
+  permission [Dead] and the offset is properly aligned. *)
+
+Definition allowed_access (m: mem) (chunk: memory_chunk) (b: block) (ofs: Z) : Prop :=
+  range_perm_neg m b ofs (ofs + size_chunk chunk) Dead
+  /\ (align_chunk chunk | ofs).
+
+Axiom allowed_access_perm:
+  forall m chunk b ofs,
+  allowed_access m chunk b ofs ->
+  ~ perm m b ofs Dead.
+
+Axiom valid_access_allowed:
+  forall m chunk b ofs,
+    valid_access m chunk b ofs ->
+    allowed_access m chunk b ofs.
 
 (** [valid_pointer m b ofs] returns [true] if the address [b, ofs]
   is nonempty in [m] and [false] if it is empty. *)
 
 Parameter valid_pointer: forall (m: mem) (b: block) (ofs: Z), bool.
 
-Axiom valid_pointer_nonempty_perm:
+Axiom valid_pointer_live_perm:
   forall m b ofs,
-  valid_pointer m b ofs = true <-> perm m b ofs Cur Nonempty.
+  valid_pointer m b ofs = true <-> perm m b ofs Live.
 Axiom valid_pointer_valid_access:
   forall m b ofs,
-  valid_pointer m b ofs = true <-> valid_access m Mint8unsigned b ofs Nonempty.
+  valid_pointer m b ofs = true <-> valid_access m Mint8unsigned b ofs.
 
 (** C allows pointers one past the last element of an array.  These are not
   valid according to the previously defined [valid_pointer]. The property
@@ -277,21 +231,22 @@ Axiom valid_pointer_implies:
 (** ** Properties of the initial memory state. *)
 
 Axiom nextblock_empty: nextblock empty = 1%positive.
-Axiom perm_empty: forall b ofs k p, ~perm empty b ofs k p.
+Axiom perm_empty: forall b ofs, ~ perm empty b ofs Live.
 Axiom valid_access_empty:
-  forall chunk b ofs p, ~valid_access empty chunk b ofs p.
+  forall chunk b ofs, ~valid_access empty chunk b ofs.
 
 (** ** Properties of [load]. *)
 
-(** A load succeeds if and only if the access is valid for reading *)
-Axiom valid_access_load:
+(** A load succeeds if the access is allowed *)
+Axiom allowed_access_load:
   forall m chunk b ofs,
-  valid_access m chunk b ofs Readable ->
+  allowed_access m chunk b ofs ->
   exists v, load chunk m b ofs = Some v.
-Axiom load_valid_access:
-  forall m chunk b ofs v,
-  load chunk m b ofs = Some v ->
-  valid_access m chunk b ofs Readable.
+(* Unclear whether disallowed accesses prevent loads. *)
+(*Axiom _access_load_md:
+  forall m chunk b ofs,
+  allowed_access m chunk b ofs ->
+  exists v, load chunk m b ofs = Some v.*)
 
 (** The value returned by [load] belongs to the type of the memory quantity
   accessed: [Vundef], [Vint] or [Vptr] for an integer quantity,
@@ -330,17 +285,17 @@ Axiom load_int16_signed_unsigned:
 
 (** ** Properties of [loadbytes]. *)
 
-(** [loadbytes] succeeds if and only if we have read permissions on the accessed
+(** [loadbytes] definitely succeeds if we have read permissions on the accessed
     memory area. *)
 
-Axiom range_perm_loadbytes:
+Axiom range_perm_loadbytes_live:
   forall m b ofs len,
-  range_perm m b ofs (ofs + len) Cur Readable ->
+  range_perm m b ofs (ofs + len) Live ->
   exists bytes, loadbytes m b ofs len = Some bytes.
-Axiom loadbytes_range_perm:
-  forall m b ofs len bytes,
-  loadbytes m b ofs len = Some bytes ->
-  range_perm m b ofs (ofs + len) Cur Readable.
+Axiom range_perm_loadbytes_md:
+  forall m b ofs len,
+  range_perm m b ofs (ofs + len) MostlyDead ->
+  exists bytes, loadbytes m b ofs len = Some bytes.
 
 (** If [loadbytes] succeeds, the corresponding [load] succeeds and
   returns a value that is determined by the
@@ -389,8 +344,7 @@ Axiom loadbytes_split:
 (** ** Properties of [store]. *)
 
 (** [store] preserves block validity, permissions, access validity, and bounds.
-  Moreover, a [store] succeeds if and only if the corresponding access
-  is valid for writing. *)
+  Moreover, a [store] succeeds if and only if the corresponding access is allowed. *)
 
 Axiom nextblock_store:
   forall chunk m1 b ofs v m2, store chunk m1 b ofs v = Some m2 ->
@@ -404,26 +358,27 @@ Axiom store_valid_block_2:
 
 Axiom perm_store_1:
   forall chunk m1 b ofs v m2, store chunk m1 b ofs v = Some m2 ->
-  forall b' ofs' k p, perm m1 b' ofs' k p -> perm m2 b' ofs' k p.
+  forall b' ofs' p, perm m1 b' ofs' p -> perm m2 b' ofs' p.
 Axiom perm_store_2:
   forall chunk m1 b ofs v m2, store chunk m1 b ofs v = Some m2 ->
-  forall b' ofs' k p, perm m2 b' ofs' k p -> perm m1 b' ofs' k p.
+  forall b' ofs' p, perm m2 b' ofs' p -> perm m1 b' ofs' p.
 
-Axiom valid_access_store:
+Axiom allowed_access_store:
   forall m1 chunk b ofs v,
-  valid_access m1 chunk b ofs Writable ->
+  allowed_access m1 chunk b ofs ->
   { m2: mem | store chunk m1 b ofs v = Some m2 }.
+Axiom disallowed_access_store:
+  forall m1 chunk b ofs v,
+  ~ allowed_access m1 chunk b ofs ->
+  store chunk m1 b ofs v = None.
 Axiom store_valid_access_1:
   forall chunk m1 b ofs v m2, store chunk m1 b ofs v = Some m2 ->
-  forall chunk' b' ofs' p,
-  valid_access m1 chunk' b' ofs' p -> valid_access m2 chunk' b' ofs' p.
+  forall chunk' b' ofs',
+  valid_access m1 chunk' b' ofs' -> valid_access m2 chunk' b' ofs'.
 Axiom store_valid_access_2:
   forall chunk m1 b ofs v m2, store chunk m1 b ofs v = Some m2 ->
-  forall chunk' b' ofs' p,
-  valid_access m2 chunk' b' ofs' p -> valid_access m1 chunk' b' ofs' p.
-Axiom store_valid_access_3:
-  forall chunk m1 b ofs v m2, store chunk m1 b ofs v = Some m2 ->
-  valid_access m1 chunk b ofs Writable.
+  forall chunk' b' ofs',
+  valid_access m2 chunk' b' ofs' -> valid_access m1 chunk' b' ofs'.
 
 (** Load-store properties. *)
 
@@ -519,27 +474,28 @@ Axiom store_int16_sign_ext:
   Moreover, a [storebytes] succeeds if and only if we have write permissions
   on the addressed memory area. *)
 
-Axiom range_perm_storebytes:
-  forall m1 b ofs bytes,
-  range_perm m1 b ofs (ofs + Z.of_nat (length bytes)) Cur Writable ->
-  { m2 : mem | storebytes m1 b ofs bytes = Some m2 }.
-Axiom storebytes_range_perm:
-  forall m1 b ofs bytes m2, storebytes m1 b ofs bytes = Some m2 ->
-  range_perm m1 b ofs (ofs + Z.of_nat (length bytes)) Cur Writable.
 Axiom perm_storebytes_1:
   forall m1 b ofs bytes m2, storebytes m1 b ofs bytes = Some m2 ->
-  forall b' ofs' k p, perm m1 b' ofs' k p -> perm m2 b' ofs' k p.
+  forall b' ofs' p, perm m1 b' ofs' p -> perm m2 b' ofs' p.
 Axiom perm_storebytes_2:
   forall m1 b ofs bytes m2, storebytes m1 b ofs bytes = Some m2 ->
-  forall b' ofs' k p, perm m2 b' ofs' k p -> perm m1 b' ofs' k p.
+  forall b' ofs' p, perm m2 b' ofs' p -> perm m1 b' ofs' p.
 Axiom storebytes_valid_access_1:
   forall m1 b ofs bytes m2, storebytes m1 b ofs bytes = Some m2 ->
-  forall chunk' b' ofs' p,
-  valid_access m1 chunk' b' ofs' p -> valid_access m2 chunk' b' ofs' p.
+  forall chunk' b' ofs',
+  valid_access m1 chunk' b' ofs' -> valid_access m2 chunk' b' ofs'.
 Axiom storebytes_valid_access_2:
   forall m1 b ofs bytes m2, storebytes m1 b ofs bytes = Some m2 ->
-  forall chunk' b' ofs' p,
-  valid_access m2 chunk' b' ofs' p -> valid_access m1 chunk' b' ofs' p.
+  forall chunk' b' ofs',
+  valid_access m2 chunk' b' ofs' -> valid_access m1 chunk' b' ofs'.
+Axiom storebytes_allowed_access_1:
+  forall m1 b ofs bytes m2, storebytes m1 b ofs bytes = Some m2 ->
+  forall chunk' b' ofs',
+  allowed_access m1 chunk' b' ofs' -> allowed_access m2 chunk' b' ofs'.
+Axiom storebytes_allowed_access_2:
+  forall m1 b ofs bytes m2, storebytes m1 b ofs bytes = Some m2 ->
+  forall chunk' b' ofs',
+  allowed_access m2 chunk' b' ofs' -> allowed_access m1 chunk' b' ofs'.
 Axiom nextblock_storebytes:
   forall m1 b ofs bytes m2, storebytes m1 b ofs bytes = Some m2 ->
   nextblock m2 = nextblock m1.
@@ -600,107 +556,93 @@ Axiom storebytes_split:
 
 (** ** Properties of [alloc]. *)
 
-(** The identifier of the freshly allocated block is the next block
-  of the initial memory state. *)
-
-Axiom alloc_result:
-  forall m1 lo hi m2 b, alloc m1 lo hi = (m2, b) ->
-  b = nextblock m1.
-
 (** Effect of [alloc] on block validity. *)
 
 Axiom nextblock_alloc:
-  forall m1 lo hi m2 b, alloc m1 lo hi = (m2, b) ->
+  forall m1 lo1 lo2 hi1 hi2 m2, alloc m1 lo1 hi1 = Some (m2, lo2, hi2) ->
   nextblock m2 = Pos.succ (nextblock m1).
 
 Axiom valid_block_alloc:
-  forall m1 lo hi m2 b, alloc m1 lo hi = (m2, b) ->
+  forall m1 lo1 lo2 hi1 hi2 m2, alloc m1 lo1 hi1 = Some (m2, lo2, hi2) ->
   forall b', valid_block m1 b' -> valid_block m2 b'.
-Axiom fresh_block_alloc:
-  forall m1 lo hi m2 b, alloc m1 lo hi = (m2, b) ->
-  ~(valid_block m1 b).
+
 Axiom valid_new_block:
-  forall m1 lo hi m2 b, alloc m1 lo hi = (m2, b) ->
-  valid_block m2 b.
+  forall m1 lo1 lo2 hi1 hi2 m2 b, alloc m1 lo1 hi1 = Some (m2, lo2, hi2) ->
+  b = nextblock m1 -> valid_block m2 b.
 Axiom valid_block_alloc_inv:
-  forall m1 lo hi m2 b, alloc m1 lo hi = (m2, b) ->
+  forall m1 lo1 lo2 hi1 hi2 m2 b, alloc m1 lo1 hi1 = Some (m2, lo2, hi2) ->
+  b = nextblock m1 ->
   forall b', valid_block m2 b' -> b' = b \/ valid_block m1 b'.
 
 (** Effect of [alloc] on permissions. *)
 
-Axiom perm_alloc_1:
-  forall m1 lo hi m2 b, alloc m1 lo hi = (m2, b) ->
-  forall b' ofs k p, perm m1 b' ofs k p -> perm m2 b' ofs k p.
+(*Axiom perm_alloc_1:
+  forall m1 lo1 lo2 hi1 hi2 m2, alloc m1 lo1 hi1 = Some (m2, lo2, hi2) ->
+  forall b' ofs p, perm m1 b' ofs p -> perm m2 b' ofs p.
 Axiom perm_alloc_2:
-  forall m1 lo hi m2 b, alloc m1 lo hi = (m2, b) ->
-  forall ofs k, lo <= ofs < hi -> perm m2 b ofs k Freeable.
-Axiom perm_alloc_3:
-  forall m1 lo hi m2 b, alloc m1 lo hi = (m2, b) ->
-  forall ofs k p, perm m2 b ofs k p -> lo <= ofs < hi.
-Axiom perm_alloc_4:
-  forall m1 lo hi m2 b, alloc m1 lo hi = (m2, b) ->
-  forall b' ofs k p, perm m2 b' ofs k p -> b' <> b -> perm m1 b' ofs k p.
+  forall m1 lo1 lo2 hi1 hi2 m2 b, alloc m1 lo1 hi1 = Some (m2, lo2, hi2) ->
+  forall ofs, lo2 <= ofs < hi2 -> perm m2 b ofs Live.
 Axiom perm_alloc_inv:
-  forall m1 lo hi m2 b, alloc m1 lo hi = (m2, b) ->
-  forall b' ofs k p,
-  perm m2 b' ofs k p ->
-  if eq_block b' b then lo <= ofs < hi else perm m1 b' ofs k p.
+  forall m1 lo1 lo2 hi1 hi2 m2, alloc m1 lo1 hi1 = Some (m2, lo2, hi2) ->
+  forall b' ofs p,
+  perm m2 b' ofs p ->
+  lo2 <= ofs < hi2 \/ perm m1 b' ofs p.
 
 (** Effect of [alloc] on access validity. *)
 
 Axiom valid_access_alloc_other:
-  forall m1 lo hi m2 b, alloc m1 lo hi = (m2, b) ->
-  forall chunk b' ofs p,
-  valid_access m1 chunk b' ofs p ->
-  valid_access m2 chunk b' ofs p.
+  forall m1 lo1 lo2 hi1 hi2 m2, alloc m1 lo1 hi1 = Some (m2, lo2, hi2) ->
+  forall chunk b' ofs,
+  valid_access m1 chunk b' ofs ->
+  valid_access m2 chunk b' ofs.
 Axiom valid_access_alloc_same:
-  forall m1 lo hi m2 b, alloc m1 lo hi = (m2, b) ->
+  forall m1 lo1 lo2 hi1 hi2 m2, alloc m1 lo1 hi1 = Some (m2, lo2, hi2) ->
   forall chunk ofs,
-  lo <= ofs -> ofs + size_chunk chunk <= hi -> (align_chunk chunk | ofs) ->
-  valid_access m2 chunk b ofs Freeable.
+  lo2 <= ofs -> ofs + size_chunk chunk <= hi2 -> (align_chunk chunk | ofs) ->
+  valid_access m2 chunk (nextblock m1) ofs.
 Axiom valid_access_alloc_inv:
-  forall m1 lo hi m2 b, alloc m1 lo hi = (m2, b) ->
-  forall chunk b' ofs p,
-  valid_access m2 chunk b' ofs p ->
+  forall m1 lo1 lo2 hi1 hi2 m2 b, alloc m1 lo1 hi1 = Some (m2, lo2, hi2) ->
+  forall chunk b' ofs,
+  valid_access m2 chunk b' ofs ->
   if eq_block b' b
-  then lo <= ofs /\ ofs + size_chunk chunk <= hi /\ (align_chunk chunk | ofs)
-  else valid_access m1 chunk b' ofs p.
+  then lo2 <= ofs /\ ofs + size_chunk chunk <= hi2 /\ (align_chunk chunk | ofs)
+  else valid_access m1 chunk b' ofs.
 
 (** Load-alloc properties. *)
 
 Axiom load_alloc_unchanged:
-  forall m1 lo hi m2 b, alloc m1 lo hi = (m2, b) ->
+  forall m1 lo1 lo2 hi1 hi2 m2, alloc m1 lo1 hi1 = Some (m2, lo2, hi2) ->
   forall chunk b' ofs,
   valid_block m1 b' ->
   load chunk m2 b' ofs = load chunk m1 b' ofs.
 Axiom load_alloc_other:
-  forall m1 lo hi m2 b, alloc m1 lo hi = (m2, b) ->
+  forall m1 lo1 lo2 hi1 hi2 m2, alloc m1 lo1 hi1 = Some (m2, lo2, hi2) ->
   forall chunk b' ofs v,
   load chunk m1 b' ofs = Some v ->
   load chunk m2 b' ofs = Some v.
 Axiom load_alloc_same:
-  forall m1 lo hi m2 b, alloc m1 lo hi = (m2, b) ->
+  forall m1 lo1 lo2 hi1 hi2 m2 b, alloc m1 lo1 hi1 = Some (m2, lo2, hi2) ->
   forall chunk ofs v,
   load chunk m2 b ofs = Some v ->
   v = Vundef.
 Axiom load_alloc_same':
-  forall m1 lo hi m2 b, alloc m1 lo hi = (m2, b) ->
+  forall m1 lo1 lo2 hi1 hi2 m2, alloc m1 lo1 hi1 = Some (m2, lo2, hi2) ->
   forall chunk ofs,
-  lo <= ofs -> ofs + size_chunk chunk <= hi -> (align_chunk chunk | ofs) ->
-  load chunk m2 b ofs = Some Vundef.
-
+  lo2 <= ofs -> ofs + size_chunk chunk <= hi2 -> (align_chunk chunk | ofs) ->
+  load chunk m2 (nextblock m1) ofs = Some Vundef.
+*)
 (** ** Properties of [free]. *)
 
 (** [free] succeeds if and only if the correspond range of addresses
-  has [Freeable] current permission. *)
+  has [Live] current permission. *)
 
 Axiom range_perm_free:
   forall m1 b lo hi,
-  range_perm m1 b lo hi Cur Freeable ->
+  range_perm m1 b lo hi Live ->
   { m2: mem | free m1 b lo hi = Some m2 }.
 Axiom free_range_perm:
   forall m1 bf lo hi m2, free m1 bf lo hi = Some m2 ->
-  range_perm m1 bf lo hi Cur Freeable.
+  range_perm m1 bf lo hi Live.
 
 (** Block validity is preserved by [free]. *)
 
@@ -715,43 +657,43 @@ Axiom valid_block_free_2:
   forall b, valid_block m2 b -> valid_block m1 b.
 
 (** Effect of [free] on permissions. *)
-
-Axiom perm_free_1:
+(*
+Axiom` perm_free_1:
   forall m1 bf lo hi m2, free m1 bf lo hi = Some m2 ->
-  forall b ofs k p,
+  forall b ofs p,
   b <> bf \/ ofs < lo \/ hi <= ofs ->
-  perm m1 b ofs k p ->
-  perm m2 b ofs k p.
+  perm m1 b ofs p ->
+  perm m2 b ofs p.
 Axiom perm_free_2:
   forall m1 bf lo hi m2, free m1 bf lo hi = Some m2 ->
-  forall ofs k p, lo <= ofs < hi -> ~ perm m2 bf ofs k p.
+  forall ofs, lo <= ofs < hi -> perm m2 bf ofs MostlyDead.
 Axiom perm_free_3:
   forall m1 bf lo hi m2, free m1 bf lo hi = Some m2 ->
-  forall b ofs k p,
-  perm m2 b ofs k p -> perm m1 b ofs k p.
+  forall b ofs p,
+  perm m2 b ofs p -> perm m1 b ofs p.
 
 (** Effect of [free] on access validity. *)
 
 Axiom valid_access_free_1:
   forall m1 bf lo hi m2, free m1 bf lo hi = Some m2 ->
-  forall chunk b ofs p,
-  valid_access m1 chunk b ofs p ->
+  forall chunk b ofs,
+  valid_access m1 chunk b ofs ->
   b <> bf \/ lo >= hi \/ ofs + size_chunk chunk <= lo \/ hi <= ofs ->
-  valid_access m2 chunk b ofs p.
+  valid_access m2 chunk b ofs.
 Axiom valid_access_free_2:
   forall m1 bf lo hi m2, free m1 bf lo hi = Some m2 ->
-  forall chunk ofs p,
+  forall chunk ofs,
   lo < hi -> ofs + size_chunk chunk > lo -> ofs < hi ->
-  ~(valid_access m2 chunk bf ofs p).
+  ~(valid_access m2 chunk bf ofs).
 Axiom valid_access_free_inv_1:
   forall m1 bf lo hi m2, free m1 bf lo hi = Some m2 ->
-  forall chunk b ofs p,
-  valid_access m2 chunk b ofs p ->
-  valid_access m1 chunk b ofs p.
+  forall chunk b ofs,
+  valid_access m2 chunk b ofs ->
+  valid_access m1 chunk b ofs.
 Axiom valid_access_free_inv_2:
   forall m1 bf lo hi m2, free m1 bf lo hi = Some m2 ->
-  forall chunk ofs p,
-  valid_access m2 chunk bf ofs p ->
+  forall chunk ofs,
+  valid_access m2 chunk bf ofs ->
   lo >= hi \/ ofs + size_chunk chunk <= lo \/ hi <= ofs.
 
 (** Load-free properties *)
@@ -761,44 +703,6 @@ Axiom load_free:
   forall chunk b ofs,
   b <> bf \/ lo >= hi \/ ofs + size_chunk chunk <= lo \/ hi <= ofs ->
   load chunk m2 b ofs = load chunk m1 b ofs.
-
-(** ** Properties of [drop_perm]. *)
-
-Axiom nextblock_drop:
-  forall m b lo hi p m', drop_perm m b lo hi p = Some m' ->
-  nextblock m' = nextblock m.
-Axiom drop_perm_valid_block_1:
-  forall m b lo hi p m', drop_perm m b lo hi p = Some m' ->
-  forall b', valid_block m b' -> valid_block m' b'.
-Axiom drop_perm_valid_block_2:
-  forall m b lo hi p m', drop_perm m b lo hi p = Some m' ->
-  forall b', valid_block m' b' -> valid_block m b'.
-
-Axiom range_perm_drop_1:
-  forall m b lo hi p m', drop_perm m b lo hi p = Some m' ->
-  range_perm m b lo hi Cur Freeable.
-Axiom range_perm_drop_2:
-  forall m b lo hi p,
-  range_perm m b lo hi Cur Freeable -> { m' | drop_perm m b lo hi p = Some m' }.
-
-Axiom perm_drop_1:
-  forall m b lo hi p m', drop_perm m b lo hi p = Some m' ->
-  forall ofs k, lo <= ofs < hi -> perm m' b ofs k p.
-Axiom perm_drop_2:
-  forall m b lo hi p m', drop_perm m b lo hi p = Some m' ->
-  forall ofs k p', lo <= ofs < hi -> perm m' b ofs k p' -> perm_order p p'.
-Axiom perm_drop_3:
-  forall m b lo hi p m', drop_perm m b lo hi p = Some m' ->
-  forall b' ofs k p', b' <> b \/ ofs < lo \/ hi <= ofs -> perm m b' ofs k p' -> perm m' b' ofs k p'.
-Axiom perm_drop_4:
-  forall m b lo hi p m', drop_perm m b lo hi p = Some m' ->
-  forall b' ofs k p', perm m' b' ofs k p' -> perm m b' ofs k p'.
-
-Axiom load_drop:
-  forall m b lo hi p m', drop_perm m b lo hi p = Some m' ->
-  forall chunk b' ofs,
-  b' <> b \/ ofs + size_chunk chunk <= lo \/ hi <= ofs \/ perm_order p Readable ->
-  load chunk m' b' ofs = load chunk m b' ofs.
 
 (** * Relating two memory states. *)
 
@@ -847,7 +751,7 @@ Axiom store_outside_extends:
   forall chunk m1 m2 b ofs v m2',
   extends m1 m2 ->
   store chunk m2 b ofs v = Some m2' ->
-  (forall ofs', perm m1 b ofs' Cur Readable -> ofs <= ofs' < ofs + size_chunk chunk -> False) ->
+  (forall ofs', perm m1 b ofs' Live -> ofs <= ofs' < ofs + size_chunk chunk -> False) ->
   extends m1 m2'.
 
 Axiom storev_extends:
@@ -873,16 +777,16 @@ Axiom storebytes_outside_extends:
   forall m1 m2 b ofs bytes2 m2',
   extends m1 m2 ->
   storebytes m2 b ofs bytes2 = Some m2' ->
-  (forall ofs', perm m1 b ofs' Cur Readable -> ofs <= ofs' < ofs + Z.of_nat (length bytes2) -> False) ->
+  (forall ofs', perm m1 b ofs' Live -> ofs <= ofs' < ofs + Z.of_nat (length bytes2) -> False) ->
   extends m1 m2'.
 
 Axiom alloc_extends:
-  forall m1 m2 lo1 hi1 b m1' lo2 hi2,
+  forall m1 m2 lo1 lo1' hi1 hi1' m1' lo2 lo2' hi2 hi2',
   extends m1 m2 ->
-  alloc m1 lo1 hi1 = (m1', b) ->
+  alloc m1 lo1 hi1 = Some (m1', lo1', hi1') ->
   lo2 <= lo1 -> hi1 <= hi2 ->
   exists m2',
-     alloc m2 lo2 hi2 = (m2', b)
+     alloc m2 lo2 hi2 = Some (m2', lo2', hi2')
   /\ extends m1' m2'.
 
 Axiom free_left_extends:
@@ -895,7 +799,7 @@ Axiom free_right_extends:
   forall m1 m2 b lo hi m2',
   extends m1 m2 ->
   free m2 b lo hi = Some m2' ->
-  (forall ofs k p, perm m1 b ofs k p -> lo <= ofs < hi -> False) ->
+  (forall ofs p, perm m1 b ofs p -> lo <= ofs < hi -> False) ->
   extends m1 m2'.
 
 Axiom free_parallel_extends:
@@ -911,11 +815,11 @@ Axiom valid_block_extends:
   extends m1 m2 ->
   (valid_block m1 b <-> valid_block m2 b).
 Axiom perm_extends:
-  forall m1 m2 b ofs k p,
-  extends m1 m2 -> perm m1 b ofs k p -> perm m2 b ofs k p.
+  forall m1 m2 b ofs p,
+  extends m1 m2 -> perm m1 b ofs p -> perm m2 b ofs p.
 Axiom valid_access_extends:
-  forall m1 m2 chunk b ofs p,
-  extends m1 m2 -> valid_access m1 chunk b ofs p -> valid_access m2 chunk b ofs p.
+  forall m1 m2 chunk b ofs,
+  extends m1 m2 -> valid_access m1 chunk b ofs -> valid_access m2 chunk b ofs.
 Axiom valid_pointer_extends:
   forall m1 m2 b ofs,
   extends m1 m2 -> valid_pointer m1 b ofs = true -> valid_pointer m2 b ofs = true.
@@ -955,17 +859,17 @@ Axiom valid_block_inject_2:
   valid_block m2 b2.
 
 Axiom perm_inject:
-  forall f m1 m2 b1 b2 delta ofs k p,
+  forall f m1 m2 b1 b2 delta ofs p,
   f b1 = Some(b2, delta) ->
   inject f m1 m2 ->
-  perm m1 b1 ofs k p -> perm m2 b2 (ofs + delta) k p.
+  perm m1 b1 ofs p -> perm m2 b2 (ofs + delta) p.
 
 Axiom valid_access_inject:
-  forall f m1 m2 chunk b1 ofs b2 delta p,
+  forall f m1 m2 chunk b1 ofs b2 delta,
   f b1 = Some(b2, delta) ->
   inject f m1 m2 ->
-  valid_access m1 chunk b1 ofs p ->
-  valid_access m2 chunk b2 (ofs + delta) p.
+  valid_access m1 chunk b1 ofs ->
+  valid_access m2 chunk b2 (ofs + delta).
 
 Axiom valid_pointer_inject:
   forall f m1 m2 b1 ofs b2 delta,
@@ -984,7 +888,7 @@ Axiom weak_valid_pointer_inject:
 Axiom address_inject:
   forall f m1 m2 b1 ofs1 b2 delta p,
   inject f m1 m2 ->
-  perm m1 b1 (Ptrofs.unsigned ofs1) Cur p ->
+  perm m1 b1 (Ptrofs.unsigned ofs1) p ->
   f b1 = Some (b2, delta) ->
   Ptrofs.unsigned (Ptrofs.add ofs1 (Ptrofs.repr delta)) = Ptrofs.unsigned ofs1 + delta.
 
@@ -1022,8 +926,8 @@ Axiom inject_no_overlap:
   b1 <> b2 ->
   f b1 = Some (b1', delta1) ->
   f b2 = Some (b2', delta2) ->
-  perm m1 b1 ofs1 Max Nonempty ->
-  perm m1 b2 ofs2 Max Nonempty ->
+  perm m1 b1 ofs1 Live ->
+  perm m1 b2 ofs2 Live ->
   b1' <> b2' \/ ofs1 + delta1 <> ofs2 + delta2.
 
 Axiom different_pointers_inject:
@@ -1082,7 +986,7 @@ Axiom store_outside_inject:
   inject f m1 m2 ->
   (forall b' delta ofs',
     f b' = Some(b, delta) ->
-    perm m1 b' ofs' Cur Readable ->
+    perm m1 b' ofs' Live ->
     ofs <= ofs' + delta < ofs + size_chunk chunk -> False) ->
   store chunk m2 b ofs v = Some m2' ->
   inject f m1 m2'.
@@ -1118,21 +1022,21 @@ Axiom storebytes_outside_inject:
   inject f m1 m2 ->
   (forall b' delta ofs',
     f b' = Some(b, delta) ->
-    perm m1 b' ofs' Cur Readable ->
+    perm m1 b' ofs' Live ->
     ofs <= ofs' + delta < ofs + Z.of_nat (length bytes2) -> False) ->
   storebytes m2 b ofs bytes2 = Some m2' ->
   inject f m1 m2'.
 
 Axiom alloc_right_inject:
-  forall f m1 m2 lo hi b2 m2',
+  forall f m1 m2 lo1 lo2 hi1 hi2 m2',
   inject f m1 m2 ->
-  alloc m2 lo hi = (m2', b2) ->
+  alloc m2 lo1 hi1 = Some (m2', lo2, hi2) ->
   inject f m1 m2'.
 
 Axiom alloc_left_unmapped_inject:
-  forall f m1 m2 lo hi m1' b1,
+  forall f m1 m2 lo1 lo2 hi1 hi2 m1' b1,
   inject f m1 m2 ->
-  alloc m1 lo hi = (m1', b1) ->
+  alloc m1 lo1 hi1 = Some (m1', lo2, hi2) ->
   exists f',
      inject f' m1' m2
   /\ inject_incr f f'
@@ -1143,18 +1047,18 @@ Definition inj_offset_aligned (delta: Z) (size: Z) : Prop :=
   forall chunk, size_chunk chunk <= size -> (align_chunk chunk | delta).
 
 Axiom alloc_left_mapped_inject:
-  forall f m1 m2 lo hi m1' b1 b2 delta,
+  forall f m1 m2 lo1 lo2 hi1 hi2 m1' b1 b2 delta,
   inject f m1 m2 ->
-  alloc m1 lo hi = (m1', b1) ->
+  alloc m1 lo1 hi1 = Some (m1', lo2, hi2) ->
   valid_block m2 b2 ->
   0 <= delta <= Ptrofs.max_unsigned ->
-  (forall ofs k p, perm m2 b2 ofs k p -> delta = 0 \/ 0 <= ofs < Ptrofs.max_unsigned) ->
-  (forall ofs k p, lo <= ofs < hi -> perm m2 b2 (ofs + delta) k p) ->
-  inj_offset_aligned delta (hi-lo) ->
-  (forall b delta' ofs k p,
+  (forall ofs p, perm m2 b2 ofs p -> delta = 0 \/ 0 <= ofs < Ptrofs.max_unsigned) ->
+  (forall ofs p, lo1 <= ofs < hi1 -> perm m2 b2 (ofs + delta) p) ->
+  inj_offset_aligned delta (hi1-lo1) ->
+  (forall b delta' ofs p,
    f b = Some (b2, delta') ->
-   perm m1 b ofs k p ->
-   lo + delta <= ofs + delta' < hi + delta -> False) ->
+   perm m1 b ofs p ->
+   lo1 + delta <= ofs + delta' < hi1 + delta -> False) ->
   exists f',
      inject f' m1' m2
   /\ inject_incr f f'
@@ -1162,12 +1066,12 @@ Axiom alloc_left_mapped_inject:
   /\ (forall b, b <> b1 -> f' b = f b).
 
 Axiom alloc_parallel_inject:
-  forall f m1 m2 lo1 hi1 m1' b1 lo2 hi2,
+  forall f m1 m2 lo1 lo1' hi1 hi1' m1' b1 lo2 lo2' hi2 hi2',
   inject f m1 m2 ->
-  alloc m1 lo1 hi1 = (m1', b1) ->
+  alloc m1 lo1 hi1 = Some (m1', lo1', hi1') ->
   lo2 <= lo1 -> hi1 <= hi2 ->
   exists f', exists m2', exists b2,
-  alloc m2 lo2 hi2 = (m2', b2)
+  alloc m2 lo2 hi2 = Some (m2', lo2', hi2')
   /\ inject f' m1' m2'
   /\ inject_incr f f'
   /\ f' b1 = Some(b2, 0)
@@ -1178,8 +1082,8 @@ Axiom free_inject:
   inject f m1 m2 ->
   free_list m1 l = Some m1' ->
   free m2 b lo hi = Some m2' ->
-  (forall b1 delta ofs k p,
-    f b1 = Some(b, delta) -> perm m1 b1 ofs k p -> lo <= ofs + delta < hi ->
+  (forall b1 delta ofs p,
+    f b1 = Some(b, delta) -> perm m1 b1 ofs p -> lo <= ofs + delta < hi ->
     exists lo1, exists hi1, In (b1, lo1, hi1) l /\ lo1 <= ofs < hi1) ->
   inject f m1' m2'.
 
@@ -1191,15 +1095,6 @@ Axiom free_parallel_inject:
   exists m2',
      free m2 b' (lo + delta) (hi + delta) = Some m2'
   /\ inject f m1' m2'.
-
-Axiom drop_outside_inject:
-  forall f m1 m2 b lo hi p m2',
-  inject f m1 m2 ->
-  drop_perm m2 b lo hi p = Some m2' ->
-  (forall b' delta ofs k p,
-    f b' = Some(b, delta) ->
-    perm m1 b' ofs k p -> lo <= ofs + delta < hi -> False) ->
-  inject f m1 m2'.
 
 (** Memory states that inject into themselves. *)
 
@@ -1216,8 +1111,8 @@ Axiom empty_inject_neutral:
   forall thr, inject_neutral thr empty.
 
 Axiom alloc_inject_neutral:
-  forall thr m lo hi b m',
-  alloc m lo hi = (m', b) ->
+  forall thr m lo1 lo2 hi1 hi2 m',
+  alloc m lo1 hi1 = Some (m', lo2, hi2) ->
   inject_neutral thr m ->
   Plt (nextblock m) thr ->
   inject_neutral thr m'.
@@ -1229,12 +1124,5 @@ Axiom store_inject_neutral:
   Plt b thr ->
   Val.inject (flat_inj thr) v v ->
   inject_neutral thr m'.
-
-Axiom drop_inject_neutral:
-  forall m b lo hi p m' thr,
-  drop_perm m b lo hi p = Some m' ->
-  inject_neutral thr m ->
-  Plt b thr ->
-  inject_neutral thr m'.
-
+*)
 End MEM.
